verif/btrees/verif_splitnode_part1.v
@@ -17,28 +17,6 @@ Require Import verif_splitnode_part0.
 
 Opaque Znth.
 
-Lemma Zlength_sublist_hack:
-  forall {X: Type} i j (al: list X),
-    i <= j ->
-    Zlength (sublist i j al) <= j-i.
-Proof.
-intros.
-unfold sublist.
-rewrite Zlength_correct.
-assert (j = (j-i) + i) by omega.
-assert (0 <= (j-i)) by omega.
-forget (j-i) as k.
-subst j.
-rewrite <- (Z2Nat.id k) in H by omega.
-rewrite <- (Z2Nat.id k) at 2 by omega.
-clear H1.
-forget (Z.to_nat k) as k'; clear k; rename k' into k.
-clear H.
-forget (Z.to_nat i) as j.
-apply Nat2Z.inj_le.
-apply firstn_le_length.
-Qed.
-
 Lemma splitnode_main_if_part2_proof:
  forall (Espec : OracleKind) (ptr0 : option (node val)) (le : list (entry val))
           (First Last : bool) (nval pe : val) (gv : globals) (v_allEntries : val)
@@ -57,8 +35,8 @@ Lemma splitnode_main_if_part2_proof:
          (H3 : Zlength allent_end = Fanout + 1 - fri)
          (FRIRANGE : 0 <= fri <= Fanout)
          (H5 : key_repr ke = key_repr k)
-         (H4 : 0 <= fri < Zlength (map entry_val_rep (nth_first_le le fri) ++ allent_end))
-         (FRILENGTH : Zlength (nth_first_le le fri) = fri),
+         (H4 : 0 <= fri < Zlength (map entry_val_rep (sublist 0 fri le) ++ allent_end))
+         (FRILENGTH : Zlength (sublist 0 fri le) = fri),
 semax (func_tycontext f_splitnode Vprog Gprog [])
   (EX ent_end : list (val * (val + val)),
    PROP (fri <= Fanout <= Fanout;
@@ -71,9 +49,9 @@ semax (func_tycontext f_splitnode Vprog Gprog [])
    btnode_rep (empty_node true false Last vnewnode);
    data_at Ews tentry (Vptrofs (Ptrofs.repr (k_ k)), inr xe) pe;
    data_at Tsh (tarray tentry 16)
-     (map entry_val_rep (nth_first_le le fri) ++
+     (map entry_val_rep (sublist 0 fri le) ++
       (Vptrofs (Ptrofs.repr (k_ k)), inr (force_val (sem_cast_pointer xe)))
-      :: map entry_val_rep (suble fri Fanout le) ++ ent_end) v_allEntries;
+      :: map entry_val_rep (sublist fri Fanout le) ++ ent_end) v_allEntries;
    entry_rep (keyval val ke ve xe))) splitnode_main_if_part2
   (frame_ret_assert
      (function_body_ret_assert tvoid
@@ -106,9 +84,14 @@ Proof.
     unfold nleft. Intros ent_end0.
     forward.                    (* node->numKeys=8 *)
     sep_apply insert_rep. fold e.
-    rewrite le_split with (le:=insert_le le e) (i:=Middle) by
-        (simpl in H0; rewrite Zlength_insert_le; rewrite H0; rewrite Middle_eq; rewrite Fanout_eq; omega).
-    rewrite iter_sepcon_app.
+    replace (insert_le le e) with 
+      (sublist 0 Middle (insert_le le e) 
+      ++ sublist Middle (Zlength (insert_le le e)) (insert_le le e)).
+    2:{ autorewrite with sublist in H4.
+         rewrite sublist_rejoin; try rep_omega.
+         autorewrite with sublist. auto.
+         simpl in H0; rewrite Zlength_insert_le, H0. rep_omega. }
+   rewrite iter_sepcon_app.
     
     forward_if (PROP ( )
     LOCAL (temp _newNode vnewnode; temp _tgtIdx (Vint (Int.repr fri));
@@ -116,10 +99,10 @@ Proof.
     SEP (mem_mgr gv; btnode_rep (splitnode_left n e); btnode_rep (empty_node true false Last vnewnode);
          data_at Ews tentry (Vptrofs (Ptrofs.repr (k_ k)), inr xe) pe;
          data_at Tsh (tarray tentry 16) 
-            (map entry_val_rep (nth_first_le le fri)
+            (map entry_val_rep (sublist 0 fri le)
              ++ (Vptrofs (Ptrofs.repr (k_ k)), inr (force_val (sem_cast_pointer xe))) 
-              :: map entry_val_rep (suble fri Fanout le) ++ ent_end) v_allEntries;
-          iter_sepcon entry_rep (skipn_le (insert_le le e) Middle))).
+              :: map entry_val_rep (sublist fri Fanout le) ++ ent_end) v_allEntries;
+          iter_sepcon entry_rep (sublist Middle (Zlength (insert_le le e)) (insert_le le e)))).
     {                           (* fri < 8 *)
       Intros.
       unfold Sfor.              (* both forward_loop and forward_for_simple_bound fail here *)
@@ -128,49 +111,49 @@ Proof.
 LOCAL (temp _newNode vnewnode; temp _tgtIdx (Vint (Int.repr fri));
        lvar _allEntries (tarray tentry 16) v_allEntries; temp _node nval; temp _entry pe;
       temp _i (Vint (Int.repr i)))
-SEP (mem_mgr gv; iter_sepcon entry_rep (nth_first_le (insert_le le e) Middle);
-          iter_sepcon entry_rep (skipn_le (insert_le le e) Middle); malloc_token Ews tbtnode nval;
+SEP (mem_mgr gv; iter_sepcon entry_rep (sublist 0 Middle (insert_le le e) );
+          iter_sepcon entry_rep (sublist Middle (Zlength (insert_le le e)) (insert_le le e)); malloc_token Ews tbtnode nval;
      data_at Ews tbtnode
        (Val.of_bool true,
        (Val.of_bool First,
        (Val.of_bool false,
        (Vint (Int.repr 8),
        (optionally getval nullval ptr0,
-        map entry_val_rep ( (nth_first_le (insert_le le e) i)) ++ le_end))))) nval;
+        map entry_val_rep ( (sublist 0 i (insert_le le e))) ++ le_end))))) nval;
      optionally btnode_rep emp ptr0; btnode_rep (empty_node true false Last vnewnode);
      data_at Ews tentry (Vptrofs (Ptrofs.repr (k_ k)), inr xe) pe;
      data_at Tsh (tarray tentry 16)
-       (map entry_val_rep ( (nth_first_le le fri)) ++
+       (map entry_val_rep ( (sublist 0 fri le)) ++
         (Vptrofs (Ptrofs.repr (k_ k)), inr (force_val (sem_cast_pointer xe)))
-        :: map entry_val_rep ( (suble fri Fanout le)) ++ ent_end) v_allEntries))%assert.
+        :: map entry_val_rep ( (sublist fri Fanout le)) ++ ent_end) v_allEntries))%assert.
       - Exists fri.
-        Exists (map entry_val_rep ((skipn_le le fri)) ++ ent_end0).
+        Exists (map entry_val_rep ((sublist fri (Zlength le) le)) ++ ent_end0).
         entailer!.
         set (fri := findRecordIndex n k) in *.
-        rewrite le_split with (i:=fri) (le:=le) at 1.
-        replace (nth_first_le (insert_le le e) fri) with (nth_first_le le fri).
-        rewrite map_app.
-        rewrite app_assoc. cancel.
+        apply derives_refl'; do 6 f_equal. rewrite <- app_ass. f_equal.
+        rewrite <- map_app. f_equal.
+        simpl in H0.
+        replace (sublist 0 fri (insert_le le e)) with (sublist 0 fri le).
+        rewrite sublist_rejoin; try list_solve.
+        autorewrite with sublist. auto.
         rewrite insert_fri with (fri:=fri) (key0:=ke); try auto with typeclass_instances.
-        rewrite nth_first_app_same1. auto. omega.
+        autorewrite with sublist. auto.
         apply FRI_repr. auto.
-        simpl in H0. rewrite H0. omega.
       -                         (* loop body *)
         Intros i.
         Intros le_end.             
         forward_if.
-        + assert(HINSERT: (map entry_val_rep ( (nth_first_le le fri)) 
+        + assert(HINSERT: (map entry_val_rep ( (sublist 0 fri le)) 
                                       ++ (Vptrofs (Ptrofs.repr (k_ k)), inr (force_val (sem_cast_pointer xe)))
-                                        :: map entry_val_rep ( (suble fri Fanout le)) ++ ent_end) 
+                                        :: map entry_val_rep ( (sublist fri Fanout le)) ++ ent_end) 
                        = map entry_val_rep ( (insert_le le e)) ++ ent_end).
           { rewrite insert_fri with (fri:=fri) (key0:=ke); auto with typeclass_instances.
             rewrite map_app.
-            simpl. rewrite H5.
-            rewrite suble_skip. unfold key_repr.
-            rewrite <- app_assoc. simpl.
+            simpl. rewrite H5. rewrite <- app_assoc. f_equal.
+            change (?A :: ?B ++ ?C) with ((A::B)++C).
+            f_equal. f_equal.
             unfold k_; rewrite Ptrofs.repr_unsigned; auto.
-            unfold n in H0. simpl in H0. auto.      
-            unfold e. simpl. auto.
+            f_equal. f_equal. simpl in H0; omega.
             rewrite FRI_repr with (key2:=k) by auto. auto.
           } 
           rewrite HINSERT.
@@ -184,12 +167,12 @@ SEP (mem_mgr gv; iter_sepcon entry_rep (nth_first_le (insert_le le e) Middle);
           destruct HEI as [ki [vi [xi HEI]]]. subst ei.
           assert_PROP(isptr xi).
           { apply le_iter_sepcon_split in HENTRY.
-            gather_SEP (iter_sepcon entry_rep (nth_first_le (insert_le le e) Middle))
-                       (iter_sepcon entry_rep (skipn_le (insert_le le e) Middle)).
+            gather_SEP (iter_sepcon entry_rep (sublist 0 Middle (insert_le le e)))
+                       (iter_sepcon entry_rep (sublist Middle (Zlength (insert_le le e)) (insert_le le e))).
             replace_SEP 0 ( iter_sepcon entry_rep (insert_le le e)).
-            { entailer!. rewrite le_split with (i:=Middle) (le:= (insert_le le e)) at 3.
-              rewrite iter_sepcon_app. entailer!. simpl in H0. rewrite Zlength_insert_le.
-              rewrite H0. rep_omega. }
+            { entailer!. rewrite <- iter_sepcon_app. rewrite sublist_rejoin; try list_solve.
+               autorewrite with sublist; auto.
+                rewrite Zlength_insert_le. simpl in H0; rewrite H0.  rep_omega. }
             rewrite HENTRY. simpl entry_rep. entailer!. }
           rename H11 into XIPTR.
           assert(HZNTH: forall ent_end, Znth (d:=(Vundef,inl Vundef)) i (map entry_val_rep ( (insert_le le e)) ++ ent_end) = entry_val_rep (keyval val ki vi xi)).
@@ -201,7 +184,6 @@ SEP (mem_mgr gv; iter_sepcon entry_rep (nth_first_le (insert_le le e) Middle);
             destruct H14, H1, H2, H3, H4.
             simplify_value_fits in H5. destruct H5.
             rewrite Zlength_app, Zlength_map in H5.
-            unfold nth_first_le in H5.
             pose proof (Zlength_sublist_hack 0 i (insert_le le e)).
             omega.  }            
           rename H12 into LEEND.
@@ -220,7 +202,6 @@ SEP (mem_mgr gv; iter_sepcon entry_rep (nth_first_le (insert_le le e) Middle);
                       rewrite Zlength_insert_le. simpl in H0; rewrite H0. rep_omega.
          }
           entailer!. apply derives_refl'; repeat f_equal.
-          unfold nth_first_le.
           autorewrite with sublist.
           rewrite upd_Znth_twice by list_solve.
           rewrite upd_Znth_same by list_solve.
@@ -237,12 +218,12 @@ SEP (mem_mgr gv; iter_sepcon entry_rep (nth_first_le (insert_le le e) Middle);
           forward.              (* break *)
           entailer!.
           unfold n, splitnode_left.
-          rewrite unfold_btnode_rep with (n:=btnode val ptr0 (nth_first_le (insert_le le e) Middle) true First false nval).
+          rewrite unfold_btnode_rep 
+          with (n:=btnode val ptr0 (sublist 0 Middle (insert_le le e)) true First false nval).
           Exists le_end.
-          cancel. Opaque nth_first_le. simpl.
+          cancel.  simpl.
           apply derives_refl'; repeat f_equal.
-          Transparent nth_first_le.
-          unfold nth_first_le. rewrite Zlength_sublist. rep_omega.
+          rewrite Zlength_sublist. rep_omega.
           rep_omega.  simpl in H0.  clear - H0. rewrite Zlength_insert_le. rep_omega.
     } 
     {                           (* fri >= 8 *)
@@ -252,18 +233,17 @@ SEP (mem_mgr gv; iter_sepcon entry_rep (nth_first_le (insert_le le e) Middle);
       assert((Middle <=? fri) = true).
       { clear -H8. rewrite Middle_eq. apply Z.leb_le. omega.  }
       unfold splitnode_left, n.
-      rewrite unfold_btnode_rep with (n:=btnode val ptr0 (nth_first_le (insert_le le e) Middle) true First false nval).
-      assert(SPLITLE:  le = (nth_first_le le Middle) ++ (skipn_le le Middle)).
-      { rewrite le_split with (i:=Middle) at 1. auto.
-        simpl in H0. rewrite H0. rewrite Middle_eq, Fanout_eq. omega. }
+      rewrite unfold_btnode_rep with (n:=btnode val ptr0 (sublist 0 Middle (insert_le le e)) true First false nval).
+      assert(SPLITLE:  le = (sublist 0 Middle le) ++ (sublist Middle (Zlength le) le)).
+      {simpl in H0. rewrite sublist_rejoin; try rep_omega. autorewrite with sublist; auto. }
       rewrite SPLITLE.
       rewrite map_app, <- app_assoc.
-      Exists (map entry_val_rep ( (skipn_le le Middle)) ++ ent_end0).
+      Exists (map entry_val_rep (sublist Middle (Zlength le) le) ++ ent_end0).
       simpl. cancel. 
       apply derives_refl'; do 5 f_equal.
      do 2 f_equal.
      rewrite <- SPLITLE.
-      unfold nth_first_le. rewrite Zlength_sublist; auto. rep_omega.
+     rewrite Zlength_sublist; auto. rep_omega.
       rewrite Zlength_insert_le. simpl in H0. rep_omega.
       do 3 f_equal.
       rewrite nth_first_insert with (k:=ke); auto with typeclass_instances.
@@ -274,18 +254,18 @@ SEP (mem_mgr gv; iter_sepcon entry_rep (nth_first_le (insert_le le e) Middle);
     }
     rewrite unfold_btnode_rep with (n:=empty_node true false Last vnewnode).
     simpl. Intros ent_empty.
-    assert(HINSERT: (map entry_val_rep ( (nth_first_le le fri))
+    assert(HINSERT: (map entry_val_rep ( (sublist 0 fri le))
                               ++ (Vptrofs (Ptrofs.repr (k_ k)), inr xe)
-                               :: map entry_val_rep ( (suble fri Fanout le)) ++ ent_end) 
+                               :: map entry_val_rep ( (sublist fri Fanout le)) ++ ent_end) 
                             = map entry_val_rep ( (insert_le le e)) ++ ent_end).
     { rewrite insert_fri with (fri:=fri) (key0:=ke); auto with typeclass_instances.
       rewrite map_app.
       simpl. rewrite H5.
-      rewrite suble_skip. unfold key_repr.
-      unfold n in H0. simpl in H0. rewrite <- app_assoc. simpl.
-      unfold k_; rewrite Ptrofs.repr_unsigned;  reflexivity. rep_omega.
-      simpl in H0. rewrite H0. auto.
-      unfold e. simpl. auto.
+      rewrite app_ass. f_equal.
+      change (?A :: ?B ++ ?C) with ((A::B)++C); f_equal.
+      f_equal.
+      unfold k_; rewrite Ptrofs.repr_unsigned;  reflexivity. 
+      do 2 f_equal; simpl in H0; rep_omega.
       rewrite FRI_repr with (key2:=k) by auto. auto.
     } 
     rewrite HINSERT.
@@ -298,11 +278,11 @@ SEP (mem_mgr gv; iter_sepcon entry_rep (nth_first_le (insert_le le e) Middle);
      malloc_token Ews tbtnode vnewnode;
      data_at Ews tbtnode
        (Vtrue, (Vfalse, (Val.of_bool Last, (Vint (Int.repr 0), (nullval,
-        map entry_val_rep ((suble Middle i (insert_le le e))) ++ ent_right)))))
+        map entry_val_rep ((sublist Middle i (insert_le le e))) ++ ent_right)))))
        vnewnode;
      data_at Ews tentry (Vptrofs (Ptrofs.repr (k_ k)), inr xe) pe;
      data_at Tsh (tarray tentry 16) (map entry_val_rep ( (insert_le le e)) ++ ent_end) v_allEntries;
-     iter_sepcon entry_rep (skipn_le (insert_le le e) Middle))))%assert.                             
+     iter_sepcon entry_rep (sublist Middle (Zlength(insert_le le e)) (insert_le le e)))))%assert.                             
     
     { Exists ent_empty. entailer!.
       simplify_value_fits in H11. decompose [and] H11.  simplify_value_fits in H23.
@@ -321,11 +301,12 @@ SEP (mem_mgr gv; iter_sepcon entry_rep (nth_first_le (insert_le le e) Middle);
       { apply le_iter_sepcon_split in HENTRY.
         rewrite unfold_btnode_rep with (n:=splitnode_left n e).
         unfold splitnode_left. unfold n. Intros ent_left.
-        gather_SEP (iter_sepcon entry_rep (nth_first_le (insert_le le e) Middle)) (iter_sepcon entry_rep (skipn_le (insert_le le e) Middle)).
+        gather_SEP (iter_sepcon entry_rep (sublist 0 Middle (insert_le le e))) 
+                          (iter_sepcon entry_rep (sublist Middle _ (insert_le le e))).
         replace_SEP 0 ( iter_sepcon entry_rep (insert_le le e)).
-        { entailer!. rewrite le_split with (i:=Middle) (le:= (insert_le le e)) at 3.
-          rewrite iter_sepcon_app. entailer!. simpl in H0. rewrite Zlength_insert_le.
-          rewrite H0. rep_omega.  }
+        { entailer!. rewrite <- iter_sepcon_app. rewrite sublist_rejoin; try rep_omega.
+           autorewrite with sublist; auto.
+          simpl in H0. rewrite Zlength_insert_le. rep_omega. }
         rewrite HENTRY. simpl entry_rep. entailer!. }
       rename H9 into XIPTR.
       assert(HZNTH: forall ent_end, Znth (d:=(Vundef,inl Vundef)) i (map entry_val_rep ( (insert_le le e)) ++ ent_end) = entry_val_rep (keyval val ki vi xi)).
@@ -355,7 +336,7 @@ SEP (mem_mgr gv; iter_sepcon entry_rep (nth_first_le (insert_le le e) Middle);
       rewrite upd_Znth_app2.
       rewrite !Zlength_map.
       apply derives_refl'. do 6 f_equal.
-      unfold suble. autorewrite with sublist.
+      autorewrite with sublist.
       rewrite Zlength_sublist; try rep_omega.
       replace (i - 8 - (i - Middle)) with 0 by rep_omega.
       rewrite upd_Znth0. fold (Z.succ i).
@@ -369,7 +350,6 @@ SEP (mem_mgr gv; iter_sepcon entry_rep (nth_first_le (insert_le le e) Middle);
       rewrite Zlength_insert_le. simpl in H0. rewrite H0. rep_omega.
       rewrite Zlength_insert_le. simpl in H0. rewrite H0. rep_omega.
       rewrite Zlength_insert_le. simpl in H0. rewrite H0. rep_omega.
-      unfold suble.
       pose proof (Zlength_insert_le _ le e). autorewrite with sublist.
       pose proof (Zlength_sublist_hack Middle i (insert_le le e)).
       spec H21; [rep_omega|].
@@ -386,17 +366,14 @@ SEP (mem_mgr gv; iter_sepcon entry_rep (nth_first_le (insert_le le e) Middle);
     change emp with (optionally btnode_rep emp ptr1).
      rewrite add_repr, sub_repr.
     fold (Z.succ Fanout).
-     assert(HSUB: suble Middle (Z.succ Fanout) (insert_le le e) = skipn_le (insert_le le e) Middle).
-      { apply suble_skip; [rep_omega|]. rewrite Zlength_insert_le. unfold n in H0. simpl in H0. rewrite H0.
-        auto.  }
-    rewrite HSUB.
+    replace (Z.succ Fanout) with (Zlength (insert_le le e))
+      by (rewrite Zlength_insert_le; unfold n in H0; simpl in H0; rewrite H0; auto).
     rewrite Middle_eq.
     sep_apply (fold_btnode_rep ptr1).
-    simpl. unfold skipn_le.
+    simpl.
     assert (Zlength le = Fanout) by (unfold n in H0; apply H0).
     rewrite Zlength_insert_le. rewrite Zlength_sublist; try rep_omega.
     rewrite Zlength_insert_le; rep_omega.
-    clear HSUB. 
     assert(NTHENTRY: exists emid, nth_entry_le Middle (insert_le le e) = Some emid).
     { apply nth_entry_le_in_range. unfold n in H0. simpl in H0. rewrite Zlength_insert_le.
       rewrite H0. rep_omega. } 
